\documentclass[10pt]{article}
\begin{document}
\begin{quote}
\textbf{Problem:} Show that, if $n$ is a positive integer, then
\[ \sum_{i=1}^{n} i^2 = \frac{n(n+1)(2n+1)}{6}\]
\end{quote}
\textbf{Proof:
} The proof will be by induction. Let $P(n)$ be the statement
\[ \sum_{i=1}^{n} i^2 = \frac{n(n+1)(2n+1)}{6}.\]
Since $\sum_{i=1}^1 i^2 = 1 = \frac{1\cdot2\cdot 3}{6}$, $P(1)$ is true.
Assume, by induction, that $P(k)$ is true for some $k > 0$. Then,
by the associative law
of addition and the inductive assumption,
\[
\sum_{i=1}^{k+1} i^2 = \left(\sum_{i=1}^{k} i^2\right) + (k+1)^2
= \frac{k(k+1)(2k+1)}{6} + (k+1)^2. \]
By finding a common denominator and simplifying,
\[ \frac{k(k+1)(2k+1)}{6} + (k+1)^2 = \frac{k(k+1)(2k+1)}{6}+
\frac{6(k+1)^2}{6} = \frac{(k+1)[(2k^2+k)+(6k+6)]}{6}\]
Since $(2k^2+k)+(6k+2) = 2k^2 + 7k + 6 = (k+2)(2k+3) = [(k+1)+1][2(k+1)+1]$,
we have that
\[ \frac{k(k+1)(2k+1)}{6} + (k+1)^2 = \frac{(k+1)[(k+1)+1][2(k+1)+1]}{6}.\]
That is, $P(k+1)$ is true.
Therefore, since $P(1)$ is true and for $k > 0$, the truth of $P(k)$ implies the
truth of $P(k+1)$, the Principle of Mathematical
Induction implies that $P(n)$ is true for all $n > 0$. Q.E.D.
\end{document}
